mgraphs.v
@@ -1,0 +1,116 @@
+Set Implicit Arguments.
+
+Require Import ZArith List Bool.
+Require Import MSets MSetWeakList MSetRBT.
+
+Module SetFunctorList (E : OrderedType) : WSetsOn E
+  := MSetWeakList.Make E.
+
+Module SetFunctorRBT (E : OrderedType) 
+  : MSetInterface.S with Module E := E
+  := MSetRBT.Make E.
+
+Module Type RawGraph (Node : UsualOrderedType) (F : WSetsOn).
+  Notation node := Node.t.
+  Module NodeSet := F Node.
+  Notation node_set := NodeSet.t.
+
+  Parameter t : Type.
+  Parameter inv : t -> Prop.
+
+  Parameter Empty : t.
+  Parameter Empty_inv : inv Empty.
+  
+  Parameter Node :
+    forall (x : node) (adj : node_set) (g : t), t.
+  Parameter Node_inv :
+    forall x adj g,
+      inv g ->
+      inv (Node x adj g).
+
+  Parameter ind :
+    forall P : t -> Prop,
+      P Empty ->
+      (forall (n : node) (adj : node_set) (g : t),
+          inv g -> P g -> P (Node n adj g)) ->
+      forall g : t, inv g -> P g.
+End RawGraph.
+
+Require Import POrderedType.
+Require Import graphs.
+
+Lemma NoDup_NoDupA_eq :
+  forall (A : Type) (l : list A),
+    NoDup l <-> NoDupA eq l.
+Proof.
+  induction l;
+  try solve[split; intros; constructor].
+  split; inversion 1; subst; constructor; auto.
+  { intros H4. rewrite InA_alt in H4.
+    destruct H4 as [y [H5 H6]]. subst a. contradiction. }
+  rewrite <-IHl; auto.
+  intros H4. apply In_InA with (eqA:=eq) in H4. contradiction.
+  apply eq_equivalence.
+  rewrite IHl; auto.
+Qed.  
+
+Module InductiveRawGraph : RawGraph Positive_as_OT MSetWeakList.Make.
+  Module NodeSet := MSetWeakList.Make Positive_as_OT.
+  Notation node_set := NodeSet.t.
+
+  Inductive graph_NoDup : graph -> Prop :=
+  | EmptyNoDup : graph_NoDup Empty
+  | NodeNoDup :
+      forall x adj g,
+        NoDup adj ->
+        graph_NoDup g -> 
+        graph_NoDup (Node x adj g). 
+
+  Definition t := graph.
+  Definition inv := graph_NoDup.
+
+  Definition Empty := Empty.
+
+  Lemma Empty_inv : inv Empty. Proof. apply EmptyNoDup. Qed.
+
+  Definition Node (x : node) (adj : node_set) (g : t) :=
+    Node x (NodeSet.this adj) g.
+
+  Lemma Node_inv :
+    forall x adj g,
+      inv g ->
+      inv (Node x adj g).
+  Proof.
+    intros x adj g H0.
+    apply NodeNoDup; auto.
+    generalize (NodeSet.is_ok adj).
+    unfold NodeSet.Raw.Ok. generalize (NodeSet.this adj) as l.
+    intros l H. rewrite NoDup_NoDupA_eq. auto.
+  Qed.    
+  
+  Lemma ind :
+    forall P : t -> Prop,
+      P Empty ->
+      (forall (n : node) (adj : node_set) (g : t),
+          inv g -> P g -> P (Node n adj g)) ->
+      forall g : t, inv g -> P g.
+  Proof.
+    intros P H IH g H2.
+    revert H2.
+    set (X := fun g => inv g -> P g).
+    change (X g).
+    apply graph_ind; unfold X; auto.
+    intros n l g' H3.
+    inversion 1; subst.
+    unfold Node in IH.
+    assert (H7: NodeSet.Raw.Ok l).
+    { unfold NodeSet.Raw.Ok.
+      rewrite <-NoDup_NoDupA_eq; apply H4. }
+    set (l' := NodeSet.Mkt l).
+    inversion H0; subst.
+    apply (IH n l' g' H9); auto.
+  Qed.
+End InductiveRawGraph.
+  
+  
+  
